Let us prove by induction on n the following statement for all n positive or negative.

STATEMENT S(n): There are integers a and b (positive or negative) such that n = 5a + 7b.

Basis: 
* For n = 0; 5(0) + 7(0) = 0;
* For n = 1; 5(3) + 7(-2) = 1;
* For n = 2; 5(-1) + 7(1) = 2;
* For n = 3; 5(2) + 7(-1) = 3;
* For n = 4; 5(-2) + 7(2) = 4;

Let us prove by induction on n the statement for all positive n.
We assume that k-2 can be presented as 5a + 7b. We suppose that if k-2 can be written as 5a + 7b then k+3 can also be written as 5a + 7b. Let's prove this.

k+3 = (k - 2) + 5;

k+3 = (5a + 7b) + 5;

k+3 = 5(a + 1) + 7b;

(a + 1) and b are integers. So k+3 can be presented as 5a + 7b. We have proved by complete induction that if the statement S(k-2) is true then the statement S(k+3) is also true.

Let us prove by induction on n the statement for all negative n.
We assume that k+3 can be presented as 5a + 7b. We suppose that if k+3 can be written as 5a + 7b then k-2 can also be written as 5a + 7b. Let's prove this.

k-2 = (k + 3) - 5;

k-2 = (5a + 7b) - 5;

k-2 = 5(a - 1) + 7b;

(a - 1) and b are integers. So k-2 can be presented as 5a + 7b. We have proved by complete induction that if the statement S(k+3) is true then the statement S(k-2) is also true.
